@prefix rdf: <http://www.w3.org/1999/02/22-rdf-syntax-ns#>.
@prefix rdfs: <http://www.w3.org/2000/01/rdf-schema#>.

:Transformation
    a rdfs:Class,
    rdfs:comment "The class of composite conceptual transformations of a transformation algebra.".

:step
    a rdf:Property;
    rdfs:comment "Constituent steps of a transformation in terms of the data that is conceptualized along the way.";
    rdfs:domain :Transformation;
    rdfs:range :Data.

:result
    a rdf:Property;
    rdfs:comment "Identifies the target data: the final output data of a transformation as a whole.";
    rdfs:domain :Transformation;
    rdfs:range :TransformedData.


:Data
    a rdfs:Class;
    rdfs:comment "The class of data instances that are conceptualized at some point during a transformation.".

:SourceData
    a rdfs:Class;
    rdfs:subClassOf :Data.

:TransformedData
    a rdfs:Class;
    rdfs:subClassOf :Data.

:InternalData
    a rdfs:Class;
    rdfs:subClassOf :Data
    rdfs:comment "Data produced by some internal process for which the structure is unknown. For example, when an operation *g* is passed as a parameter to some other operation *f*, the data produced by *g* within *f* may be preprocessed by unknown internals.".

:origin
    a rdf:Property;
    rdfs:comment "Identifies the node that represents the source of some input data.";
    rdfs:domain :SourceData.

:feeds
    a rdf:Property;
    rdfs:comment "Connects input data to the transformed data that is based on it.";
    rdfs:domain :Data;
    rdfs:range :TransformedData.

:transformer
    a rdf:Property;
    rdfs:comment "The conceptual operation by which the data was transformed.";
    rdfs:domain :TransformedData;
    rdfs:range :Operation.

:internal
    a rdf:Property;
    rdfs:comment "Indicate that the transformer that produced this data is involved in some internal process.";
    rdfs:domain :TransformedData;
    rdfs:range :InternalData.


:Operation
    a rdfs:Class;
    rdfs:comment "The class of atomary conceptual transformations.".


:Type
    a rdfs:Class;
    rdfs:comment "The class of all transformation types.".

:Function
    a rdfs:Class;
    rdfs:subClassOf :TypeOperator;
    rdfs:comment "The class of function types.".
