
:transformation
    rdfs:comment "The object is a transformation represented by the subject.",
    rdfs:range :Transformation.

:Transformation
    a rdfs:Class,
    rdfs:comment "The class of full transformations.".

:operation
    rdfs:comment "A constituent operation of a transformation.",
    rdfs:domain :Transformation,
    rdfs:range :Operation.

:data
    rdfs:comment "Some input, intermediary or output data of a transformation.",
    rdfs:domain :Transformation,
    rdfs:range :Data.

:Operation
    a rdfs:Class,
    rdfs:comment "The class of operations, representing the atomary constituents of conceptual transformations.".

:Data
    a rdfs:Class,
    rdfs:comment "The class of data (input, output or intermediary) relevant to conceptual transformations.".

:Variable
    a rdfs:Class,
    rdfs:comment "A node representing variable data or operation.".

:source
    rdfs:comment "The source for some input data.",
    rdfs:domain :Data.

:input
    rdfs:comment "The input data for a transformation.",
    rdfs:domain :Operation,
    rdfs:range :Data.

:output
    rdfs:comment "The output data for a transformation.",
    rdfs:domain :Operation,
    rdfs:range :Data.

# Types.
:type
    rdfs:comment "A .",
    rdfs:domain :Data,
    rdfs:range :Type.
:Type
    a rdfs:Class,
    rdfs:comment "The class of all types".
:TypeVariable
    rdfs:comment "The class of type variables.",
    a :Type.
:TypeOperator
    rdfs:comment "The class of concrete types.",
    a :Type.
:Function
    rdfs:comment "The class of type operations for functions.";
    a :TypeOperator.
